$(a+b)(a+b)=(a+b)^2$
$(a+b)^2=a^2+b^2-2ab$
$(a-b)(a-b)= (a-b)^2$
$a^2-b^2= (a+b)(a-b)$

Conjugate

**Question 2:**


$3(4+3i)-2(3-2i)= 12+9i-6+4i$
$6+13i$
$\dfrac{4+3i}{3-2i}$

Multiply by a fraction of the conjugate of the denominator
$\therefore \dfrac{4+3i}{3-2i} \cdot \dfrac{3+2i}{3+2i}$

$\dfrac{12+8i+9i+6i^2}{3^2-(2i)^2}$
$\dfrac{6+17i}{13}$

$\dfrac{Z_{2}}{Z_{1}}=\dfrac{3-2i}{4+3i}$
$\therefore \bar{Z_{1}}=4-3i$
$\dfrac{3-2i}{4+3i}\cdot\dfrac{4-3i}{4-3i}$
$\dfrac{12-9i-8i+6i^2}{4^2-(3i)^2}=\dfrac{6-17i}{25}$
**vi)**
$\dfrac{Z_{1}-1}{Z_{2}+i}=\dfrac{3+3i}{3-i}$
$\dfrac{3+3i}{3-i}\cdot\dfrac{3+i}{3+i}$
$\dfrac{9+3i+9i+3i^2}{10}$
$\dfrac{6+12i}{10}=\dfrac{3+6i}{5}$


**IX)**
$(Z_{1}-Z_{2})^2$
$((4+3i)-(3-2i))^2$
$(i+5i)^2$
$1+25i^2+10i$


**X)**
$Z_{1}^{-1}\cdot Z_{2}^{-1}=\dfrac{1}{Z_{1}}\cdot\dfrac{1}{Z_{2}}$

for $Z_{1}$
$\dfrac{1}{Z_{1}}=\dfrac{1}{4+3i}\cdot\dfrac{4-3i}{4-3i}$
$=\dfrac{4-3i}{4^2-(3i)^2}$
$= \dfrac{4-3i}{25}$

for $Z_{2}$
$\dfrac{1}{Z_{2}}=\dfrac{1}{3-2i}\cdot\dfrac{3+2i}{3+2i}$
$=\dfrac{3+2i}{3^2-(2i)^2}$
$=\dfrac{3+2i}{13}$

$\therefore \dfrac{1}{Z_{1}}\cdot\dfrac{1}{Z_{2}} = \dfrac{4-3i}{25}\cdot\dfrac{3+2i}{13}$
$=\dfrac{12+8i-9i-6i^2}{325}$
$=\dfrac{18-i}{325}$




**Question 7:**
$7\sqrt{ 2 }\cdot\text{cis}(-45\degree)$
$7\sqrt{ 2 }\cdot(\cos(-45\degree) + i \sin(-45\degree))$
$7\sqrt{ 2 }\cdot((\dfrac{\sqrt{ 2 }}{2}) + i (\dfrac{-\sqrt{ 2 }}{2}))$
$7\sqrt{ 2 }\cdot(1-i)\dfrac{\sqrt{ 2 }}{2}$
$7-7i$

# Practice

[[Practice Tutorial 3.pdf]]

$u=1-i$ and $v=-\sqrt{ 3 }+1$

**II)**


$2\sqrt{ 3 }u-\sqrt{ 3 }v$
$2\sqrt{ 3 }(1-i)-\sqrt{ 3 }(-\sqrt{ 3 }+1)$
$3\sqrt{ 3 }i-9$