$v=u+at$
$s=ut+\dfrac{1}{2}at^2$
$v^2=u^2-2as$
$s=vt$

# SUVAT Equations


|             |    **WITHOUT**     |            **WITHOUT**            |            **WITHOUT**            |      **WITHOUT**      |       **WITHOUT**       |
| ----------- | :----------------: | :-------------------------------: | :-------------------------------: | :-------------------: | :---------------------: |
| **SUBJECT** |      **$s$**       |      $s=vt-\dfrac{1}{2}at^2$      |      $s=ut+\dfrac{1}{2}at^2$      | $s=\dfrac{t}{2}(u+v)$ | $s=\dfrac{u^2+v^2}{2a}$ |
| **SUBJECT** |      $u=v-at$      |                $u$                |      $u=\dfrac{s-at^2}{2t}$       |  $u=\dfrac{2s}{t}+v$  |  $u=\sqrt{ 2as-v^2 }$   |
| **SUBJECT** |      $v=u+at$      |      $v=\dfrac{s+at^2}{2t}$       |                $v$                |  $v=\dfrac{2s}{t}-u$  |  $v=\sqrt{ u^2+2as }$   |
| **SUBJECT** | $a=\dfrac{v-u}{t}$ |      $a=\dfrac{2(vt-s)}{2t}$      |     $a=\dfrac{2(s-ut)}{t^2}$      |          $a$          | $a=\dfrac{v^2-u^2}{2s}$ |
| **SUBJECT** | $t=\dfrac{v-u}{a}$ | $t=\dfrac{v-\sqrt{ v^2-2as }}{a}$ | $t=\dfrac{\sqrt{ 2as+u^2 }-u}{a}$ |  $t=\dfrac{2s}{u+v}$  |           $t$           |
